
$$
f(x)=P_n(x)+R_n(x)
$$

$$
\begin{align}
P_n(x_0)&=f(x_0)+f'(x_0)(x-x_0)+\frac {f''(x_0)(x-x_0)^2}{2!}+\cdots +\frac{f^{(n)}(x_0)(x-x_0)^n}{n!}\\
&=\sum^{n}_{k=0}\frac{f^{(k)}(x_0)}{k!}(x-x_0)^n\\
R_n(x)&=\frac{f^{(n+1)}(\xi)}{(n+1)!}(x-x_0)^{n+1}\quad ,其中\xi\in(x_0,x)
\end{align}
$$

$$
\begin{align}
\frac{R_n(x)}{{(x-x_0)}^{n+1}}=\frac{R_n(x)-R_n(x_0)}{{(x-x_0)}^{n+1}-0}&=\frac {R'_n(\xi)}{(n+1)(\xi-x_0)}=\cdots=\frac{R^{(n+1)}_n(\xi)}{(n+1)!}=\frac{f^{(n+1)}_n(\xi)}{(n+1)!}\\
&\uparrow求导（洛必达）
\end{align}
$$

$$
f(x)=1+x+\frac{x^2}{2}+\frac{x^3}{3!}+\cdots+\frac{x^{n}}{n!}+o(x^n)
$$

